Modified typing rule in STLC

stlc.v
@@ -47,9 +47,9 @@ Inductive simplto : Exp.t -> Exp.t -> Prop :=
 Hint Constructors simplto.
 
 Inductive typed : list Types.t -> Exp.t -> Types.t -> Prop :=
-  | T_Var : forall env x d,
-      x < length env ->
-      typed env (Exp.Var x) (nth x env d)
+  | T_Var : forall env x t,
+      nth x (map Some env) None = Some t ->
+      typed env (Exp.Var x) t
   | T_Abs : forall env e t1 t2,
       typed (t1 :: env) e t2 ->
       typed env (Exp.Abs t1 e) (Types.Fun t1 t2)
@@ -59,19 +59,6 @@ Inductive typed : list Types.t -> Exp.t -> Types.t -> Prop :=
       typed env (Exp.App e1 e2) t2.
 Hint Constructors typed.
 
-Lemma typed_weakening : forall env env' e t,
-  typed env e t ->
-  typed (env ++ env') e t.
-Proof.
-  intros ? ? ? ? Htyped.
-  induction Htyped; eauto.
-
-  erewrite <- app_nth1 by omega.
-  econstructor.
-  rewrite app_length.
-  omega.
-Qed.
-
 Lemma typed_shift : forall env e t,
   typed env e t ->
   forall env' env'' env''',
@@ -80,21 +67,43 @@ Lemma typed_shift : forall env e t,
 Proof.
   intros ? ? ? Htyped.
   induction Htyped; intros env' env'' env''' ?; subst; simpl; eauto.
-  - destruct (lt_dec x (length env')).
-    + rewrite app_nth1 by omega.
-      apply typed_weakening.
-      auto.
-    + replace (nth x (env' ++ env''') d)
-      with (nth (length env'' + x) (env' ++ env'' ++ env''') d).
-      * constructor.
-        repeat rewrite app_length in *.
-        omega.
-      * repeat rewrite app_nth2 by omega.
-        f_equal.
-        omega.
+  - destruct (lt_dec x (length env')); econstructor; repeat rewrite map_app in *.
+    + rewrite app_nth1 in * by (rewrite map_length; omega).
+      assumption.
+    + repeat rewrite app_nth2 in * by (repeat rewrite map_length; omega).
+      repeat rewrite map_length in *.
+      replace (length env'' + x - length env' - length env'')
+      with (x - length env') by omega.
+      assumption.
   - constructor.
     apply (IHHtyped (t1 :: env')).
-    eauto.
+    reflexivity.
+Qed.
+
+Lemma substitution : forall e t env,
+  typed env e t ->
+  forall env' t' env'' v,
+  env = env' ++ t' :: env'' ->
+  typed env'' v t' ->
+  typed (env' ++ env'') (Exp.subst (length env') [v] e) t.
+Proof.
+  intros ? ? ? Htyped.
+  induction Htyped; intros env' ? ? ? ? ?; subst; simpl in *; eauto.
+  - rewrite map_app in *.
+    destruct (le_dec (length env') x).
+    + rewrite app_nth2 in * by (rewrite map_length; omega).
+      eapply typed_shift with (env' := []); [| reflexivity ].
+      rewrite map_length in *.
+      remember (x - length env') as y.
+      destruct y; simpl in *.
+      * congruence.
+      * destruct y; rewrite <- minus_n_O; eauto.
+    + econstructor.
+      rewrite map_app.
+      repeat rewrite app_nth1 in * by (rewrite map_length; omega).
+      assumption.
+  - constructor.
+    eapply (IHHtyped (t1 :: env')); simpl; eauto.
 Qed.
 
 Lemma canonical_form_fun : forall v t1 t2,
@@ -102,32 +111,8 @@ Lemma canonical_form_fun : forall v t1 t2,
   typed [] v (Types.Fun t1 t2) ->
   exists e, v = Exp.Abs t1 e.
 Proof.
-  intros ? ? ? Hvalue Htyped.
-  inversion Hvalue; subst; inversion Htyped; eauto.
-Qed.
-
-Lemma substitution : forall e1 t1 env,
-  typed env e1 t1 ->
-  forall env' env'' e2 t2,
-  env = env' ++ t2 :: env'' ->
-  typed env'' e2 t2 ->
-  typed (env' ++ env'') (Exp.subst (length env') [e2] e1) t1.
-Proof.
-  intros ? ? ? Htyped.
-  induction Htyped; intros env' ? ? ? ? Htyped'; subst; simpl in *; eauto.
-  - destruct (le_dec (length env') x); rewrite app_length in *; simpl in *.
-    + rewrite app_nth2 by omega.
-      eapply typed_shift with (env' := []); [| reflexivity ].
-      remember (x - length env') as y.
-      destruct y as [| y ].
-      * eauto.
-      * destruct y; simpl; constructor; omega.
-    + rewrite app_nth1 by omega.
-      apply typed_weakening.
-      constructor.
-      omega.
-  - constructor.
-    eapply (IHHtyped (t1 :: env')); simpl; eauto.
+  intros ? ? ? Hv Htyped.
+  inversion Hv; subst; inversion Htyped; eauto.
 Qed.
 
 Lemma preservation : forall e e',
@@ -138,9 +123,10 @@ Lemma preservation : forall e e',
 Proof.
   intros ? ? Hsimplto.
   induction Hsimplto; intros ? ? Htyped; inversion Htyped; eauto.
-  
+
   inversion H3.
-  eapply substitution with (env' := []); [| reflexivity |]; eauto.
+  eapply substitution with (env' := []); eauto.
+  reflexivity.
 Qed.
 
 Lemma progress : forall e t,
@@ -150,7 +136,7 @@ Proof.
   intros ? ? Htyped.
   remember [] as env.
   induction Htyped; subst; simpl in *; eauto.
-  - omega.
+  - destruct x; congruence.
   - destruct (IHHtyped1 eq_refl) as [| []]; [| eauto ].
     destruct (canonical_form_fun _ _ _ H Htyped1).
     subst.
